theories/multiple_updates.v
@@ -568,26 +568,4 @@ Section std_updates.
            +++ rewrite /= lookup_insert_ne in Hy;auto. rewrite Hx0 in Hy; inversion Hy; subst; left.
   Qed.*)
 
-  (* TODO move in the appropriate section *)
-  Lemma related_sts_pub_world_revoked_permanent W a :
-    (std W) !! a = Some Revoked →
-    related_sts_pub_world W (<s[a:=Permanent]s>W).
-  Proof.
-    intros Ha.
-    rewrite /related_sts_pub_world /=.
-    split;[|apply related_sts_pub_refl].
-    rewrite /related_sts_pub. split.
-    - rewrite dom_insert_L. set_solver.
-    - intros i x y Hx Hy.
-      destruct (decide (a = i)).
-      + subst.
-        rewrite Hx in Ha. inversion Ha.
-        rewrite lookup_insert in Hy. inversion Hy.
-        right with (Permanent);[|left]. constructor.
-      + rewrite lookup_insert_ne in Hy;auto.
-        rewrite Hx in Hy.
-        inversion Hy; subst.
-        left.
-  Qed.
-
 End std_updates.
